proof/completeness.v
@@ -1,4 +1,4 @@
-Require Import algo.ott.
+(* Require Import algo.ott.
 Require Import decl.ott.
 Require Import transfer.
 
@@ -6,3 +6,5 @@ Require Import transfer.
 Theorem completeness : forall Γ', ld_worklist_reducible Γ' -> exists Γ, transfer' Γ Γ' /\ la_worklist_reducible Γ.
 Proof.
 Admitted.
+
+ *)
