proof/ln_utils.v
@@ -1,0 +1,34 @@
+
+Require Export Metalib.Metatheory.
+
+
+Ltac inst_cofinite_impl H x :=
+  match type of H with
+  | forall x, x `notin` ?L -> _ =>
+      let Fr := fresh "Fr" in
+      assert (x `notin` L) as Fr by auto;
+      specialize (H x Fr); clear Fr
+  end
+.
+
+Ltac inst_cofinites_with x :=
+  repeat
+    match goal with
+    | H : forall x0, x0 `notin` ?L -> _ |- _ =>
+      inst_cofinite_impl H x
+    end
+.
+
+Ltac inst_cofinites :=
+  match goal with
+  | x : atom |- _ => inst_cofinites_with x
+  end.
+
+Ltac inst_cofinites_with_new :=
+  let x := fresh "x" in
+  pick fresh x; inst_cofinites_with x.
+
+Ltac inst_cofinites_by F :=
+  let L := F in
+  let x := fresh "x" in
+  pick fresh x for L; inst_cofinites_with x.
