proof/soundness.v
@@ -5,11 +5,19 @@ Require Import decl.ott.
 Require Import transfer.
 
 
-Theorem soundness : forall Γ, la_worklist_reducible Γ -> exists Γ', transfer' Γ Γ' /\ ld_worklist_reducible Γ'.
+Theorem soundness : forall Γ, la_worklist_reducible Γ -> exists Γ', transfer Γ Γ' /\ ld_worklist_reducible Γ'.
 Proof.
   intros. induction H.
   - destruct IHla_worklist_reducible as [dwl Hdwl]. destruct Hdwl.
     exists (ld_wl_cons_tv dwl x5). split. 
     + dependent destruction H1. econstructor. econstructor. eauto.
     + econstructor; eauto. simpl. econstructor. admit. admit.
+  - destruct IHla_worklist_reducible as [dwl Hdwl]. destruct Hdwl. 
+    destruct tl.
+    + simpl in *. exists dwl. split. 
+      * unfold transfer in H1. destruct H1 as [θ'].
+        exists (cons (pair ex5 (sse_ev ld_t_int)) θ'). eapply inst_wl_ev; eauto.
+        admit. constructor.
+      * auto.
+    +
 Admitted.
